PiLL/PiLL/Framework/Model/Base.lean
@@ -33,11 +33,23 @@ class HasOpen (Subject Replacement Target : Type) where
 notation:max S:max "⸨" T " | " R "⸩" => HasOpen.open_ S R T
 notation:max S:max "⸨" R "⸩" => HasOpen.open_ S R 0
 
+class HasClose (Subject Replacement Target : Type) where
+  close_ : Subject → Replacement → Target → Subject
+
+notation:max S:max "⟦" T " | " R "⟧" => HasOpen.close_ S R T
+notation:max S:max "⟦" R "⟧" => HasOpen.close_ S R 0
+
 class HasOpenTwo (Subject Replacement_1 Replacement_2 Target : Type) where
   open_ : Subject → Replacement_1 → Replacement_2 → Target → Subject
 
 notation:max S:max "⸨" T " | " R1 ", " R2 "⸩" => HasOpenTwo.open_ S R1 R2 T
 notation:max S:max "⸨" R1 ", " R2 "⸩" => HasOpenTwo.open_ S R1 R2 0
+
+class HasCloseTwo (Subject Replacement_1 Replacement_2 Target : Type) where
+  close_ : Subject → Replacement_1 → Replacement_2 → Target → Subject
+
+notation:max S:max "⟦" T " | " R1 ", " R2 "⟧" => HasOpenTwo.open_ S R1 R2 T
+notation:max S:max "⟦" R1 ", " R2 "⟧" => HasOpenTwo.open_ S R1 R2 0
 
 class HasBracket (Subject Content Result : Type) where
    brack : Subject → Content → Result
